LwRust/Paper/Soundness/Lemma_4_10_Progress.lean
@@ -973,7 +973,7 @@ theorem progress_typing {store : ProgramStore} {env₁ env₂ : Env}
     intro _env₁ _env₂ _env₃ _env₄ _env₅ _typing lifetime condition trueBranch
       falseBranch trueTy falseTy joinTy hcondition _htrue _hfalse _hjoin _henvJoin
       _hsameLeft _hsameRight _hwellJoin _hcontained _hcoherent _hlinear
-      _hresultSafe ihCondition _ihTrue _ihFalse hvst hwf hsafe hstore
+      ihCondition _ihTrue _ihFalse hvst hwf hsafe hstore
     rcases ihCondition hvst.ite_condition hwf hsafe hstore with
       hterminalCondition | hstepCondition
     · rcases (terminal_iff_value condition).mp hterminalCondition with
