LwRust/Paper/Soundness/Theorem_4_12_TypeAndBorrowSafety.lean
@@ -460,7 +460,7 @@ theorem reachable_progress {store store' : ProgramStore} {env₁ env₂ : Env}
     intro _env₁ _env₂ _env₃ _env₄ _env₅ _typing _lifetime _condition
       _trueBranch _falseBranch _trueTy _falseTy _joinTy _hcondition _htrue
       _hfalse _hjoin _henvJoin _hsameLeft _hsameRight _hwellJoin _hcontained
-      _hcoherent _hlinear _hresultSafe ihCondition ihTrue
+      _hcoherent _hlinear ihCondition ihTrue
       ihFalse htypingEq hsource store store' term' hvalid hvst hwf hsafe
       hfs hmulti
     cases htypingEq
